@prefix : <https://w3id.org/sepses/ns/logex#> .
@prefix log: <https://w3id.org/sepses/ns/log#> .
@prefix owl: <http://www.w3.org/2002/07/owl#> .
@prefix rdf: <http://www.w3.org/1999/02/22-rdf-syntax-ns#> .
@prefix xml: <http://www.w3.org/XML/1998/namespace> .
@prefix xsd: <http://www.w3.org/2001/XMLSchema#> .
@prefix rdfs: <http://www.w3.org/2000/01/rdf-schema#> .
@base <https://w3id.org/sepses/ns/logex#> .

<https://w3id.org/sepses/ns/logex#> rdf:type owl:Ontology ;
                                     owl:versionIRI <https://w3id.org/sepses/ns/logex/1.0.0> ;
                                     owl:imports <https://w3id.org/sepses/ns/log/1.0.0> ;
                                     <http://purl.org/dc/elements/1.1/creator> "Fajar J. Ekaputra" ;
                                     <http://purl.org/dc/elements/1.1/description> "An ontology to capture SLOGERT extraction components"@en ;
                                     <http://purl.org/dc/elements/1.1/rights> "http://creativecommons.org/licenses/by/4.0/" ;
                                     <http://purl.org/dc/elements/1.1/title> "SLOGERT log extraction ontology" ;
                                     <http://purl.org/vocab/vann/preferredNamespacePrefix> "logex" .

#################################################################
#    Object Properties
#################################################################

###  https://w3id.org/sepses/ns/logex#associatedLogSourceType
:associatedLogSourceType rdf:type owl:ObjectProperty ;
                         rdfs:domain :LogEventTemplate ;
                         rdfs:range log:SourceType ;
                         rdfs:comment "logex:LogEventTemplate can be associated with one or more log:SourceType." .


###  https://w3id.org/sepses/ns/logex#hasParameterList
:hasParameterList rdf:type owl:ObjectProperty ;
                  rdfs:domain :LogEventTemplate ;
                  rdfs:range rdf:List ;
                  rdfs:comment "a list of parameter types (as strings) extracted from slogert engine. the default parameter type is 'unknown', and a set of predefined parameter type is defined in the slogert configuration file." .


###  https://w3id.org/sepses/ns/logex#isLogEventTemplateOf
:isLogEventTemplateOf rdf:type owl:ObjectProperty ;
                      rdfs:domain :LogEventTemplate ;
                      rdfs:range log:Event ;
                      rdfs:comment "relation between logex:LogEventTemplate and log:Event that conforms to it." .


#################################################################
#    Data properties
#################################################################

###  https://w3id.org/sepses/ns/logex#example
:example rdf:type owl:DatatypeProperty ;
         rdfs:domain :LogEventTemplate ;
         rdfs:range xsd:string ;
         rdfs:comment "(random) example patterns from this template" .


###  https://w3id.org/sepses/ns/logex#keyword
:keyword rdf:type owl:DatatypeProperty ;
         rdfs:domain :LogEventTemplate ;
         rdfs:range xsd:string ;
         rdfs:comment "keywords extracted from Stanford NER engine from the template patterns" .


###  https://w3id.org/sepses/ns/logex#pattern
:pattern rdf:type owl:DatatypeProperty ;
         rdfs:domain :LogEventTemplate ;
         rdfs:range xsd:string ;
         rdfs:comment "patterns of log events as extracted from LogPai" .


#################################################################
#    Classes
#################################################################

###  http://www.w3.org/1999/02/22-rdf-syntax-ns#List
rdf:List rdf:type owl:Class .


###  https://w3id.org/sepses/ns/logex#LogEventTemplate
:LogEventTemplate rdf:type owl:Class ;
                  rdfs:comment "A class to represent a LogEventTemplate, which contains information about patterns of log:Event." .


###  Generated by the OWL API (version 4.5.6.2018-09-06T00:27:41Z) https://github.com/owlcs/owlapi
